securedrop-protocol/protocol-minimal/proofs/fstar/extraction/Securedrop_protocol_minimal.Primitives.Provider.Hkdf.fst
@@ -1,0 +1,12 @@
+module Securedrop_protocol_minimal.Primitives.Provider.Hkdf
+#set-options "--fuel 0 --ifuel 1 --z3rlimit 15"
+open FStar.Mul
+open Core_models
+
+/// HKDF-SHA256
+assume
+val sha256': okm: t_Slice u8 -> salt: t_Slice u8 -> ikm: t_Slice u8 -> info: t_Slice u8
+  -> (t_Slice u8 & Core_models.Result.t_Result Prims.unit Libcrux_hkdf.t_ExpandError)
+
+unfold
+let sha256 = sha256'
